Finally complete Inductive types (now we need the constructors)

Translation/Example.v
@@ -5,12 +5,163 @@
 From Coq Require Import Bool String List BinPos Compare_dec Omega.
 From Equations Require Import Equations DepElimDec.
 From Template Require Import Ast LiftSubst Typing Checker Template.
-From Translation Require Import SAst SLiftSubst SCommon ITyping XTyping
+From Translation Require Import SAst SLiftSubst SCommon ITyping
+                                ITypingLemmata ITypingMore XTyping
                                 Translation Reduction FinalTranslation.
 
 Open Scope string_scope.
 
+Module IT := ITyping.
+
 (*! General utilities to build ETT derivations and terms *)
+
+(** We first create a global context for ITT. *)
+
+Definition iNat :=
+  {| inductive_mind := "Coq.Init.Datatypes.nat"; inductive_ind := 0 |}.
+
+Definition sNat :=
+  sInd iNat.
+
+Definition sZero :=
+  (* For now we can't use this definition as it isn't part of our syntax. *)
+  (* sConstruct iNat 0. *)
+  sRel 0.
+
+Definition sSuc :=
+  (* sConstruct iNat 1. *)
+  sRel 0.
+
+Definition iVec :=
+  {| inductive_mind := "Translation.Quotes.vec"; inductive_ind := 0 |}.
+
+Definition sVec :=
+  sInd iVec.
+
+Definition vec_cod :=
+  sProd nAnon sNat (sSort 0).
+
+Definition vec_type :=
+  sProd (nNamed "A") (sSort 0) vec_cod.
+
+Definition lΣi := [
+  SInductiveDecl "Coq.Init.Datatypes.nat" {|
+    sind_npars := 0;
+    sind_bodies := [
+      {| sind_name := "nat";
+         sind_type := sSort 0 ;
+         sind_kelim := [InProp; InSet; InType];
+         sind_ctors := [
+           ("O", sRel 0, 0) ;
+           ("S", sProd nAnon (sRel 0) (sRel 1), 1)
+         ] ;
+         sind_projs := [] |}
+    ];
+    sind_universes :=
+      Monomorphic_ctx (pair [] {|
+        Constraint.this := [] ;
+        Constraint.is_ok := Constraint.Raw.empty_ok
+      |})
+  |} ;
+  SInductiveDecl "Coq.Init.Datatypes.bool" {|
+    sind_npars := 0;
+    sind_bodies := [
+      {| sind_name := "bool";
+         sind_type := sSort 0 ;
+         sind_kelim := [InProp; InSet; InType];
+         sind_ctors := [
+           ("true", sRel 0, 0) ;
+           ("false", sRel 0, 0)
+         ] ;
+         sind_projs := [] |}
+    ];
+    sind_universes :=
+      Monomorphic_ctx (pair [] {|
+        Constraint.this := [] ;
+        Constraint.is_ok := Constraint.Raw.empty_ok
+      |})
+  |} ;
+  SInductiveDecl "Translation.Quotes.vec" {|
+    sind_npars := 1;
+    sind_bodies := [
+      {| sind_name := "vec";
+         sind_type := vec_type ;
+         sind_kelim := [InProp; InSet; InType];
+         sind_ctors := [
+           ("vnil",
+            sProd (nNamed "A")
+                  (sSort 0)
+                  (sApp (sApp (sRel 1)
+                              (nNamed "A") (sSort 0) vec_cod
+                              (sRel 0))
+                        nAnon sNat (sSort 0)
+                        sZero),
+            0) ;
+           ("vcons",
+            sProd (nNamed "A") (sSort 0)
+                  (sProd nAnon (sRel 0)
+                         (sProd (nNamed "n") sNat
+                                (sProd nAnon
+                                       (sApp (sApp (sRel 3)
+                                                   (nNamed "A") (sSort 0)
+                                                   vec_cod
+                                                   (sRel 2))
+                                             nAnon sNat (sSort 0)
+                                             (sRel 0))
+                                       (sApp (sApp (sRel 4)
+                                                   (nNamed "A") (sSort 0)
+                                                   vec_cod
+                                                   (sRel 3))
+                                             nAnon sNat (sSort 0)
+                                             (sApp sSuc
+                                                   nAnon sNat sNat
+                                                   (sRel 1)))))),
+            3)
+         ] ;
+         sind_projs := [] |}
+    ];
+    sind_universes :=
+      Monomorphic_ctx (pair [] {|
+        Constraint.this := [] ;
+        Constraint.is_ok := Constraint.Raw.empty_ok
+      |})
+  |}
+].
+
+Definition Σi := (lΣi, init_graph).
+
+Fact hΣi : type_glob Σi.
+Proof.
+  unfold type_glob. cbn.
+  constructor.
+  - constructor.
+    + constructor.
+      * constructor.
+      * cbn. constructor.
+      * cbn. constructor.
+        -- exists (max_sort 1 1). unfold vec_type.
+           eapply IT.type_Prod.
+           ++ constructor. constructor.
+           ++ unfold vec_cod. change 1 with (max 0 1).
+              eapply IT.type_Prod.
+              ** (* Problem, are the inductives in the wrong order?? I copied from Σ though... *)
+                 admit.
+              ** constructor. econstructor.
+                 --- econstructor.
+                     +++ constructor.
+                     +++ econstructor. constructor.
+                 --- admit.
+        -- repeat constructor.
+        -- cbn. admit.
+        -- cbn. constructor.
+        -- cbn. constructor.
+    + cbn. repeat constructor. cbn. easy.
+    + admit.
+  - admit.
+  - admit.
+Admitted.
+
+(* Now some useful lemmata *)
 
 Definition pn := nNamed "pppp".
 
@@ -31,7 +182,7 @@ Fixpoint multiLam (bl : list sterm) (t : sterm) :=
 Inductive wfb : scontext -> list sterm -> Type :=
 | wfb_nil Γ : wfb Γ []
 | wfb_cons Γ A s bl :
-    Σ ;;; Γ |-x A : sSort s ->
+    Σi ;;; Γ |-x A : sSort s ->
     wfb (svass pn A :: Γ) bl ->
     wfb Γ (A :: bl).
 
@@ -39,10 +190,10 @@ Derive Signature for wfb.
 
 Lemma type_multiProd :
   forall {bl Γ},
-    wf Σ Γ ->
+    wf Σi Γ ->
     wfb Γ bl ->
     ∑ s,
-      Σ ;;; Γ |-x multiProd bl : sSort s.
+      Σi ;;; Γ |-x multiProd bl : sSort s.
 Proof.
   intro bl. induction bl ; intros Γ hwf h.
   - cbn. exists (succ_sort (succ_sort 0)). apply type_Sort. assumption.
@@ -68,11 +219,11 @@ Defined.
 Inductive wbtm : scontext -> list sterm -> sterm -> Type :=
 | wbtm_nil Γ t : wbtm Γ [] t
 | wbtm_one Γ A s t :
-    Σ ;;; Γ |-x A : sSort s ->
-    Σ ;;; Γ |-x t : A ->
+    Σi ;;; Γ |-x A : sSort s ->
+    Σi ;;; Γ |-x t : A ->
     wbtm Γ [ A ] t
 | wbtm_cons Γ A B s bl t :
-    Σ ;;; Γ |-x A : sSort s ->
+    Σi ;;; Γ |-x A : sSort s ->
     wbtm (svass pn A :: Γ) (B :: bl) t ->
     wbtm Γ (A :: B :: bl) t.
 
@@ -98,9 +249,9 @@ Defined.
 
 Lemma type_multiLam :
   forall {bl Γ t},
-    wf Σ Γ ->
+    wf Σi Γ ->
     wbtm Γ bl t ->
-    Σ ;;; Γ |-x multiLam bl t : multiProd bl.
+    Σi ;;; Γ |-x multiLam bl t : multiProd bl.
 Proof.
   intro bl. induction bl ; intros Γ t hwf hwb.
   - cbn. apply type_Sort. assumption.
@@ -128,25 +279,25 @@ Defined.
 
 Lemma type_conv'' :
   forall {Γ t A B s},
-    Σ ;;; Γ |-x t : A ->
-    Σ ;;; Γ |-x A = B : sSort s ->
-    Σ ;;; Γ |-x B : sSort s ->
-    Σ ;;; Γ |-x t : B.
+    Σi ;;; Γ |-x t : A ->
+    Σi ;;; Γ |-x A = B : sSort s ->
+    Σi ;;; Γ |-x B : sSort s ->
+    Σi ;;; Γ |-x t : B.
 Proof.
   intros Γ t A B s H H0 H1.
   eapply type_conv ; eassumption.
 Defined.
 
 Fact istrans_nil :
-  ctxtrans Σ nil nil.
+  ctxtrans Σi nil nil.
 Proof.
   split.
   - constructor.
   - constructor.
 Defined.
 
-Definition type_translation {Σ Γ t A} h {Γ'} hΓ :=
-  pi2_ _ _ (pi1_ _ _ (@complete_translation Σ)) Γ t A h Γ' hΓ.
+Definition type_translation {Γ t A} h {Γ'} hΓ :=
+  pi2_ _ _ (pi1_ _ _ (@complete_translation Σi hΣi)) Γ t A h Γ' hΓ.
 
 (*! EXAMPLE 1:
     λ A B e x ⇒ x : ∀ (A B : Type), A = B → A → B
@@ -169,7 +320,7 @@ Definition ty : sterm := multiProd tyl.
 
 Definition tm : sterm := multiLam tyl (sRel 0).
 
-Fact tmty : Σ ;;; [] |-x tm : ty.
+Fact tmty : Σi ;;; [] |-x tm : ty.
 Proof.
   eapply type_multiLam.
   - constructor.
@@ -257,7 +408,7 @@ Definition ty0 : sterm := multiProd tyl0.
 
 Definition tm0 : sterm := multiLam tyl0 (sRel 0).
 
-Lemma tmty0 : Σ ;;; [] |-x tm0 : ty0.
+Lemma tmty0 : Σi ;;; [] |-x tm0 : ty0.
 Proof.
   eapply type_multiLam.
   - constructor.
@@ -308,18 +459,27 @@ Make Definition coq_red_tm0 :=
     It gets translated to itself.
 *)
 
-Definition iNat :=
-  {| inductive_mind := "Coq.Init.Datatypes.nat"; inductive_ind := 0 |}.
+Lemma xmeta_conv :
+  forall (Σ : sglobal_context) (Γ : scontext) (t A B : sterm),
+    Σ;;; Γ |-x t : A ->
+    A = B ->
+    Σ;;; Γ |-x t : B.
+Proof.
+  intros Σ Γ t A B h e.
+  destruct e. assumption.
+Defined.
 
 Lemma natty :
-  Σ ;;; [] |-x sInd iNat 0 : sSort 0.
+  Σi ;;; [] |-x sNat : sSort 0.
 Proof.
-  eapply type_Ind.
-  - constructor.
-  - Unshelve.
-    repeat econstructor;
-    try (simpl; omega); assert(H':=type_Construct Σ Γ c i u _ _ H); simpl in H';
-    clear H; apply H'; try trivial.
+  eapply xmeta_conv.
+  - eapply type_Ind.
+    + constructor.
+    + Unshelve.
+      repeat econstructor;
+      try (simpl; omega); assert(H':=type_Construct Σ Γ c i u _ _ H); simpl in H';
+      clear H; apply H'; try trivial.
+  - cbn. reflexivity.
 Defined.
 
 Definition itt_nat : sterm.
@@ -348,3 +508,38 @@ Make Definition coq_nat :=
     vec nat 1
     We cannot even write it!
 *)
+
+Lemma vecty :
+  Σi ;;; [] |-x sVec : vec_type.
+Proof.
+  eapply xmeta_conv.
+  - eapply type_Ind.
+    + constructor.
+    + Unshelve.
+      repeat econstructor;
+      try (simpl; omega); assert(H':=type_Construct Σ Γ c i u _ _ H); simpl in H';
+      clear H; apply H'; try trivial.
+  - cbn. reflexivity.
+Defined.
+
+Definition itt_vec : sterm.
+  destruct (type_translation vecty istrans_nil) as [A [t [_ h]]].
+  exact t.
+Defined.
+
+Definition itt_vec' := ltac:(let t := eval lazy in itt_vec in exact t).
+
+Definition tc_vec : tsl_result term :=
+  tsl_rec (2 ^ 18) Σ [] itt_vec'.
+
+Definition tc_vec' := ltac:(let t := eval lazy in tc_vec in exact t).
+
+Make Definition coq_vec :=
+  ltac:(
+    let t := eval lazy in
+             (match tc_vec' with
+              | Success t => t
+              | _ => tSort Universe.type0
+              end)
+      in exact t
+  ).
